theories/examples/enclaves/mutual_attestation_spec.v
@@ -4,8 +4,9 @@ From cap_machine Require Import proofmode.
 From cap_machine Require Import mutual_attestation_code.
 From cap_machine Require Import
   mutual_attestation_code
-  mutual_attestation_A_spec
-  mutual_attestation_B_spec.
+  (* mutual_attestation_A_spec *)
+  (* mutual_attestation_B_spec *)
+.
 
 
 Section mutual_attest_main.
@@ -18,44 +19,165 @@ Section mutual_attest_main.
   (* ------------------- ENCLAVES --------------------- *)
   (* -------------------------------------------------- *)
 
-  Lemma mutual_attest_contract :
-    custom_enclave_contract ma_enclaves_map.
-  Proof.
-    rewrite /custom_enclave_contract.
-    iIntros (I b e a v b' e' a' v' enclave_data ot ce
-      Hwf_cemap Hcode_ce Hot Hb' HIhash Hb He)
-      "(#Henclaves_inv & #Hma_inv & #HPenc & #HPsign)".
-    clear HIhash.
-    clear Hwf_cemap.
-    assert (e = (b ^+ (length (code ce) + 1))%a) as -> by solve_addr+He.
+  (* Lemma mutual_attest_contract : *)
+  (*   custom_enclave_contract ma_enclaves_map. *)
+  (* Proof. *)
+  (*   rewrite /custom_enclave_contract. *)
+  (*   iIntros (I b e a v b' e' a' v' enclave_data ot ce *)
+  (*     Hwf_cemap Hcode_ce Hot Hb' HIhash Hb He) *)
+  (*     "(#Henclaves_inv & #Hma_inv & #HPenc & #HPsign)". *)
+  (*   clear HIhash. *)
+  (*   clear Hwf_cemap. *)
+  (*   assert (e = (b ^+ (length (code ce) + 1))%a) as -> by solve_addr+He. *)
 
-    rewrite /ma_enclaves_map in Hcode_ce.
-    simplify_map_eq.
+  (*   rewrite /ma_enclaves_map in Hcode_ce. *)
+  (*   simplify_map_eq. *)
 
-    assert (I = hash_mutual_attest_A \/ I = hash_mutual_attest_B) as HI.
-    { rewrite lookup_insert_Some in Hcode_ce.
-      destruct Hcode_ce as [ [? _] | [_ Hcode_ce] ]; first auto.
-      rewrite lookup_insert_Some in Hcode_ce.
-      destruct Hcode_ce as [ [? _] | [_ Hcode_ce] ]; first auto.
-      done.
-    }
-    destruct HI ; simplify_map_eq.
-    - iApply ( mutual_attest_A_contract with "[]") ; last iFrame "#"; eauto.
-    - rewrite lookup_insert_ne // in Hcode_ce.
-      2:{ rewrite /hash_mutual_attest_A /hash_mutual_attest_B.
-          intro Hcontra.
-          apply hash_concat_inj' in Hcontra.
-          destruct Hcontra as [_ Hcontra].
-          rewrite /mutual_attest_enclave_A_code /mutual_attest_enclave_B_code in Hcontra.
-          by injection Hcontra.
-      }
-      simplify_map_eq.
-      iApply ( mutual_attest_B_contract with "[]") ; last iFrame "#"; eauto.
-  Admitted.
+  (*   assert (I = hash_mutual_attest_A \/ I = hash_mutual_attest_B) as HI. *)
+  (*   { rewrite lookup_insert_Some in Hcode_ce. *)
+  (*     destruct Hcode_ce as [ [? _] | [_ Hcode_ce] ]; first auto. *)
+  (*     rewrite lookup_insert_Some in Hcode_ce. *)
+  (*     destruct Hcode_ce as [ [? _] | [_ Hcode_ce] ]; first auto. *)
+  (*     done. *)
+  (*   } *)
+  (*   destruct HI ; simplify_map_eq. *)
+  (*   - iApply ( mutual_attest_A_contract with "[]") ; last iFrame "#"; eauto. *)
+  (*   - rewrite lookup_insert_ne // in Hcode_ce. *)
+  (*     2:{ rewrite /hash_mutual_attest_A /hash_mutual_attest_B. *)
+  (*         intro Hcontra. *)
+  (*         apply hash_concat_inj' in Hcontra. *)
+  (*         destruct Hcontra as [_ Hcontra]. *)
+  (*         rewrite /mutual_attest_enclave_A_code /mutual_attest_enclave_B_code in Hcontra. *)
+  (*         by injection Hcontra. *)
+  (*     } *)
+  (*     simplify_map_eq. *)
+  (*     iApply ( mutual_attest_B_contract with "[]") ; last iFrame "#"; eauto. *)
+  (* Admitted. *)
 
   (* -------------------------------------------------- *)
   (* ---------------------- MAIN ---------------------- *)
   (* -------------------------------------------------- *)
+
+
+  Lemma mutual_attestation_main_attest_or_fail_spec
+    (pc_b pc_e pc_a : Addr) (pc_v : Version)
+    (expected_hash : Z) (r : RegName) (w w5 w6: LWord)
+    φ :
+    let code :=  mutual_attestation_main_attest_or_fail r expected_hash in
+    let otype_w := match lword_get_word w with
+                   | WSealed o _ => o
+                   | _ => (-1)%Z
+                   end
+    in
+    let pc_a' := (pc_a ^+ (length code + 1))%a in
+    (pc_a + (length code + 1))%a = Some pc_a' ->
+    SubBounds pc_b pc_e pc_a (pc_a ^+ (length code))%a ->
+
+    ( PC ↦ᵣ LCap RX pc_b pc_e pc_a pc_v
+      ∗ r ↦ᵣ w ∗ r_t5 ↦ᵣ w5 ∗ r_t6 ↦ᵣ w6
+      ∗ codefrag pc_a pc_v code
+      ∗ ▷ ( (∃ tid, ⌜ has_seal otype_w tid ⌝ ∗ enclave_all tid expected_hash
+            ∗ PC ↦ᵣ LCap RX pc_b pc_e pc_a' pc_v
+            ∗ r ↦ᵣ w ∗ (∃ w5', r_t5 ↦ᵣ w5') ∗ (∃ w6', r_t6 ↦ᵣ w6')
+            ∗ codefrag pc_a pc_v code)
+            -∗ WP Seq (Instr Executable) {{ v, ⌜ v = FailedV ⌝ ∨ φ v }}
+      )
+    )
+   ⊢ WP Seq (Instr Executable) {{ v, ⌜ v = FailedV ⌝ ∨ φ v }}.
+  Proof.
+    intros code otype_w pc_a' Hpc_a' Hbounds; subst code.
+    iIntros "(HPC & Hr & Hr5 & Hr6 & Hcode & Hφ)".
+    codefrag_facts "Hcode".
+    iInstr "Hcode".
+    { transitivity (Some otype_w); auto.
+      destruct w ; auto.
+      by destruct sb.
+    }
+
+    iInstr_lookup "Hcode" as "Hi" "Hcode".
+    wp_instr.
+    iApply (wp_estoreid_success_unknown with "[$HPC $Hr6 $Hr5 $Hi]"); try solve_pure.
+    iNext. iIntros (retv) "H".
+    iDestruct "H" as "(Hi & Hr5 & [(-> & HPC & H)|(-> & HPC & Hr6)])".
+    1: iDestruct "H" as (I tid) "(Hr6 & #Hma_env & %Hseal)".
+    all: wp_pure; iInstr_close "Hcode".
+    2:{ wp_end; by iLeft. }
+    (* iDestruct (interp_valid_sealed with "Hinterp_w1") as (Φ) "Hseal_valid". *)
+
+    iInstr "Hcode".
+    iInstr "Hcode".
+    iInstr "Hcode".
+    destruct (decide (I = expected_hash)) as [-> | HnI]
+    ; cycle 1.
+    { (* Not the right enclave *)
+      iInstr "Hcode". (* Jnz *)
+      by (injection; intro Hcontra; lia).
+      iInstr "Hcode". (* Fail *)
+      wp_end; by iLeft.
+    }
+    replace ( _ - _)%Z with 0%Z by lia.
+    iInstr "Hcode".
+    iInstr "Hcode".
+    { transitivity (Some (pc_a')); subst pc_a' ; solve_addr. }
+    iInstr "Hcode".
+    iApply "Hφ".
+    replace (pc_a ^+ (9%nat + 1))%a with pc_a' by (subst pc_a' ; solve_addr).
+    iExists tid; iFrame "∗#%".
+    iSplitL "Hr5" ; iExists _ ; iFrame.
+  Qed.
+
+  Lemma mutual_attestation_main_get_confirm_or_fail_spec
+    (pc_b pc_e pc_a : Addr) (pc_v : Version)
+    (r r' : RegName) (w w' w5 w6: LWord)
+    φ :
+    let code := mutual_attestation_main_get_confirm_or_fail r r' in
+    let pc_a' := (pc_a ^+ (length code))%a in
+    (pc_a + (length code))%a = Some pc_a' ->
+    SubBounds pc_b pc_e pc_a (pc_a ^+ (length code))%a ->
+
+    ( PC ↦ᵣ LCap RX pc_b pc_e pc_a pc_v
+      ∗ r ↦ᵣ w ∗ r' ↦ᵣ w' ∗ r_t5 ↦ᵣ w5 ∗ r_t6 ↦ᵣ w6
+      ∗ codefrag pc_a pc_v code
+      ∗ ▷ ( (PC ↦ᵣ LCap RX pc_b pc_e pc_a' pc_v
+            ∗ r ↦ᵣ w ∗ r' ↦ᵣ w' ∗ (∃ w5', r_t5 ↦ᵣ w5') ∗ (∃ w6', r_t6 ↦ᵣ w6')
+            ∗ codefrag pc_a pc_v code)
+            -∗ WP Seq (Instr Executable) {{ v, ⌜ v = FailedV ⌝ ∨ φ v }}
+      )
+    )
+   ⊢ WP Seq (Instr Executable) {{ v, ⌜ v = FailedV ⌝ ∨ φ v }}.
+  Proof.
+    intros code pc_a' Hpc_a' Hbounds; subst code.
+    iIntros "(HPC & Hr & Hr' & Hr5 & Hr6 & Hcode & Hφ)".
+    codefrag_facts "Hcode".
+    iAssert (⌜ PC ≠ r ⌝)%I as %HPCr. admit.
+    iAssert (⌜ PC ≠ r' ⌝)%I as %HPCr'. admit.
+    iAssert (⌜ r ≠ r' ⌝)%I as %Hrr'. admit.
+
+    wp_instr.
+    (* iMod (inv_acc with "Henclaves_inv") as "(Henclaves_inv_open & Hclose_inv)"; first solve_ndisj. *)
+    iInstr_lookup "Hcode" as "Hi" "Hcode".
+    iDestruct (map_of_regs_3 with "HPC Hr Hr'") as "[Hmap _]".
+    iApply (wp_UnSeal with "[$Hmap $Hi]") ; try (by simplify_map_eq) ; try solve_pure.
+    { by unfold regs_of; rewrite !dom_insert; set_solver+. }
+    iNext. iIntros (regs' retv) "(#Hspec & Hpc_a & Hmap)". iDestruct "Hspec" as %Hspec.
+    destruct Hspec as [ ? ? ? ? ? ? ? Hps Hbounds' Hregs'|]; cycle 1.
+    { (* iMod ("Hclose_inv" with "Henclaves_inv_open") as "_". iModIntro. *)
+      by wp_pure; wp_end; by iLeft.
+    }
+    (* iDestruct "Henclaves_inv_open" as (ECn) "(HEC & #Hcemap)". *)
+    (* iMod ("Hclose_inv" with "[HEC Hcemap]") as "_"; iModIntro. *)
+    (* { iExists ECn. iFrame "HEC Hcemap". } *)
+    (* Opaque mutual_attest_enclave_B_code_pre encodeInstrsLW. *)
+    incrementLPC_inv as (p''&pc_b'&pc_e'&pc_a''&pc_v'& ? & HPC & Z & Hregs');
+      simplify_map_eq.
+    repeat (rewrite insert_commute //= insert_insert).
+    (* repeat (rewrite insert_commute //= insert_insert) in H1. *)
+    (* Transparent mutual_attest_enclave_B_code_pre encodeInstrsLW. *)
+    replace x with (pc_a'' ^+ 1)%a by solve_addr.
+    clear Z.
+    iDestruct (regs_of_map_3 with "[$Hmap]") as "[HPC [Hr Hr'] ]"; eauto; iFrame.
+    wp_pure; iInstr_close "Hcode".
+
 
 
 
